<?xml version="1.0"?>
<section xml:id="recursion_calculating-the-sum-of-a-list-of-numbers">
  <title>Calculating the Sum of a List of Numbers</title>
  <p>We will begin our investigation with a simple problem that you already
            know how to solve without using recursion. Suppose that you want to
            calculate the sum of a list of numbers such as:
            <m>[1, 3, 5, 7, 9]</m>. An iterative function that computes the sum
            is shown in <xref ref="lst-itsum"/>. The function uses an accumulator variable
            (<c>the_sum</c>) to compute a running total of all the numbers in the list
            by starting with <m>0</m> and adding each number in the list.</p>
<listing  xml:id="lst-itsum">
  <program  interactive="activecode" language="python">
    <input>
def list_sum(num_list):
    the_sum = 0
    for i in num_list:
        the_sum = the_sum + i
    return the_sum

print(list_sum([1, 3, 5, 7, 9]))
        </input>
  </program>
</listing>
  <p>Pretend for a minute that you do not have <c>while</c> loops or <c>for</c>
            loops. How would you compute the sum of a list of numbers? If you were a
            mathematician you might start by recalling that addition is a function
            that is defined for two parameters, a pair of numbers. To redefine the
            problem from adding a list to adding pairs of numbers, we could rewrite
            the list as a fully parenthesized expression. Such an expression looks
            like this:</p>
  <math_block docname="Recursion/CalculatingtheSumofaListofNumbers"  nowrap="False" number="True" xml:space="preserve">((((1 + 3) + 5) + 7) + 9)</math_block>
  <p>We can also parenthesize
            the expression the other way around,</p>
  <math_block docname="Recursion/CalculatingtheSumofaListofNumbers"  nowrap="False" number="True" xml:space="preserve">(1 + (3 + (5 + (7 + 9))))</math_block>
  <p>Notice that the innermost set of
            parentheses, <m>(7 + 9)</m>, is a problem that we can solve without a
            loop or any special constructs. In fact, we can use the following
            sequence of simplifications to compute a final sum.</p>
  <math_block docname="Recursion/CalculatingtheSumofaListofNumbers"  nowrap="False" number="True" xml:space="preserve">total = \  (1 + (3 + (5 + (7 + 9)))) \\
total = \  (1 + (3 + (5 + 16))) \\
total = \  (1 + (3 + 21)) \\
total = \  (1 + 24) \\
total = \  25</math_block>
  <p>How can we take this idea and turn it into a Python program? First,
            let's restate the sum problem in terms of Python lists. We might say
            the sum of the list <c>num_list</c> is the sum of the first element of the
            list (<c>num_list[0]</c>) and the sum of the numbers in the rest of the
            list (<c>num_list[1:]</c>). To state it in a functional form:</p>
  <math_block docname="Recursion/CalculatingtheSumofaListofNumbers"  nowrap="False" number="True" xml:space="preserve">list\_sum(num\_list) = first(num\_list) + list\_sum(rest(num\_list))
\label{eqn:list_sum}</math_block>
  <p>In this equation <m>first(num\_list)</m> returns the first element of
            the list and <m>rest(num\_list)</m> returns a list of everything but
            the first element. This is easily expressed in Python as shown in
            <xref ref="lst-recsum"/>.</p>
<listing xml:id="lst-recsum">â€¨<program label="lst-recsum"   interactive="activecode" language="python">
    <input>
def list_sum(num_list):
    if len(num_list) == 1:
        return num_list[0]
    else:
        return num_list[0] + list_sum(num_list[1:])

print(list_sum([1, 3, 5, 7, 9]))
        </input>
  </program>
</listing>
  <p>There are a few key ideas in this listing to look at. First, on line 2 we are checking to see if the list is one element long. This
            check is crucial and is our escape clause from the function. The sum of
            a list of length 1 is trivial; it is just the number in the list.
            Second, on line 5 our function calls itself! This is the
            reason that we call the <c>list_sum</c> algorithm recursive. A recursive
            function is a function that calls itself.</p>
  <p><xref ref="recursion_fig-recsumin"/> shows the series of <term>recursive calls</term> that are
            needed to sum the list <m>[1, 3, 5, 7, 9]</m>. You should think of
            this series of calls as a series of simplifications. Each time we make a
            recursive call we are solving a smaller problem, until we reach the
            point where the problem cannot get any smaller.</p>

  <figure xml:id="recursion_fig-recsumin" align="center">
    <image source="Recursion/Figures/sumlistIn.png" width="50%" alt="image"/>
  </figure>
  <p>When we reach the point where the problem is as simple as it can get, we
            begin to piece together the solutions of each of the small problems
            until the initial problem is solved. <xref ref="recursion_fig-recsumout"/> shows the
            additions that are performed as <c>list_sum</c> works its way backward
            through the series of calls. When <c>list_sum</c> returns from the topmost
            problem, we have the solution to the whole problem.</p>

  <figure xml:id="recursion_fig-recsumout" align="center">
    <image source="Recursion/Figures/sumlistOut.png" width="50%" alt="image"/>
  </figure>
</section>
